\documentclass[onecolumn,11pt]{article}
\setlength{\oddsidemargin}{0in}
\setlength{\evensidemargin}{0in}
\setlength{\textwidth}{6.5in}
\setlength{\textheight}{9in}
\setlength{\topmargin}{0in}
\setlength{\headheight}{0in}
\setlength{\headsep}{0in}
\usepackage{amsfonts}
\usepackage{alltt}
\usepackage[latin1]{inputenc}
\usepackage{moreverb}
\usepackage{graphicx}
\usepackage{latexsym}
\usepackage{amsmath}
\usepackage{fullpage}
\usepackage{alltt}

\title{CS442 Assignment 2}
\author{Nissan Pow\\20187246\\npow}
\date{\today}

\newtheorem{definition}{Definition}
\newtheorem{theorem}{Theorem}
\newcommand{\nonterm}[1]{\ensuremath{\langle\mbox{\emph{#1}}\rangle}}
\newcommand{\post}[2]{\ensuremath{\frac{\begin{array}{c}#1\end{array}}{\begin{array}{c}#2\end{array}}}}
\newcommand{\sem}[1]{\ensuremath{[\![#1]\!]}}

\begin{document}
\maketitle

\section*{Part A}

\section*{Parts B and D}
\begin{alltt}
\verbatimtabinput[2]{a2qbd.scm}
\end{alltt}

\section*{Part C}

\begin{alltt}
  \verbatimtabinput[2]{transcript}
\end{alltt}

\section*{Part D}
\begin{itemize}
\item I did not need to make any modifications to the unification algorithm.
\item I chose to implement letex and handle by extending W:
 \[\post
    { \{ \langle \text{var,exception} \rangle \} + A \vdash \text{E:}\ \tau} 
    { A \vdash \text{(letex\ var E):}\ \tau }
    \text{\ [letex]}
\]

\[\post
    { \text{A} \vdash \text{E:}\ exception \qquad \text{A} \vdash \text{E2:}\ \tau \qquad \text{A} \vdash \text{E3:}\ \tau }
    { A \vdash \text{(handle E1 E2 E3):}\ \tau }
    \text{\ [handle]}
\]

\begin{alltt}
W (A, (letex var E)) = 
  let 
    <S1, tau1> = (W E ((var,exception) + A) 
  in 
    <S1, tau1)>

W (A, (handle E1 E2 E3)) =
  let
    <S1, tau1> = (W E1 A)
    S2 = U(exception, tau1)
    <S3, tau3> = (W E2 A(S2 o S1))
    <S4, tau4> = (W E3 A(S3 o S2 o S1))
    S5 = U(tau3 S4, tau4)
  in
    (S5 o S4 o S3 o S2 o S1, tau4 S5)

\end{alltt}

\item And raise as a primitive type: \\
raise: ($\forall \alpha$. exception $\to$ $\alpha$)

\end{itemize}

\section*{Part E}

\begin{enumerate}

\item 
  f : $\lambda x : \forall \alpha . \forall \beta. \alpha \rightarrow \beta. (\Lambda \beta. \Lambda \alpha ((x\{\alpha\})\{\beta\})) : (\forall \alpha . \forall \beta . \alpha \rightarrow \beta) \rightarrow (\forall \beta. \forall \alpha. \alpha \rightarrow \beta) $ \\
  g : $\lambda x : \forall \beta . \forall \alpha. \alpha \rightarrow \beta. (\Lambda \alpha. \Lambda \beta ((x\{\beta\})\{\alpha\})): (\forall \beta . \forall \alpha . \alpha \rightarrow \beta) \rightarrow (\forall \alpha. \forall \beta. \alpha \rightarrow \beta) $

\item 

\[
\post
{ \post
  { \post
    { \post
      { \post
        { \post
          { \{\langle x, \forall \alpha. \forall \beta. \alpha \rightarrow \beta \rangle \}(x)  = \forall \alpha. \forall \beta. \alpha \rightarrow \beta }
          { \{\langle x, \forall \alpha. \forall \beta. \alpha \rightarrow \beta \rangle \} \vdash x : \forall \alpha. \forall \beta . \alpha \rightarrow \beta } [var]
        } 
        { \{\langle x, \forall \alpha. \forall \beta. \alpha \rightarrow \beta \rangle \} \vdash x\{\alpha\} : \forall \beta.\alpha \rightarrow \beta } [spec]
      }
      { \{\langle x, \forall \alpha. \forall \beta. \alpha \rightarrow \beta \rangle \} \vdash (x\{\alpha\})\{\beta\} : \alpha \rightarrow \beta } [spec]
    }
    { \{\langle x, \forall \alpha. \forall \beta. \alpha \rightarrow \beta \rangle \} \vdash \Lambda \alpha . ((x\{\alpha\})\{\beta\}) : \forall \alpha . \alpha \rightarrow \beta } [gen]
  }
 { \{\langle x, \forall \alpha. \forall \beta. \alpha \rightarrow \beta \rangle \} \vdash \Lambda \beta. \Lambda \alpha. ((x\{\alpha\})\{\beta\}) : \forall \beta. \forall \alpha. \alpha \rightarrow \beta } [gen]
}
{ \{\} \vdash \lambda x : \forall \alpha . \forall \beta. \alpha \rightarrow \beta. (\Lambda \beta. \Lambda \alpha ((x\{\alpha\})\{\beta\})): (\forall \alpha . \forall \beta . \alpha \rightarrow \beta) \rightarrow (\forall \beta. \forall \alpha. \alpha \rightarrow \beta) } [t-abs]
\]

\[
\post
{ \post
  { \post
    { \post
      { \post
        { \post
          { \{\langle x, \forall \beta. \forall \alpha. \alpha \rightarrow \beta \rangle \}(x)  = \forall \beta. \forall \alpha. \alpha \rightarrow \beta }
          { \{\langle x, \forall \beta. \forall \alpha. \alpha \rightarrow \beta \rangle \} \vdash x : \forall \beta. \forall \alpha . \alpha \rightarrow \beta } [var]
        } 
        { \{\langle x, \forall \beta. \forall \alpha. \alpha \rightarrow \beta \rangle \} \vdash x\{\beta\} : \forall \alpha.\alpha \rightarrow \beta } [spec]
      }
      { \{\langle x, \forall \beta. \forall \alpha. \alpha \rightarrow \beta \rangle \} \vdash (x\{\beta\})\{\alpha\} : \alpha \rightarrow \beta } [spec]
    }
    { \{\langle x, \forall \beta. \forall \alpha. \alpha \rightarrow \beta \rangle \} \vdash \Lambda \beta . ((x\{\beta\})\{\alpha\}) : \forall \beta . \alpha \rightarrow \beta } [gen]
  }
 { \{\langle x, \forall \beta. \forall \alpha. \alpha \rightarrow \beta \rangle \} \vdash \Lambda \alpha. \Lambda \beta. ((x\{\beta\})\{\alpha\}) : \forall \alpha. \forall \beta. \alpha \rightarrow \beta } [gen]
}
{ \{\} \vdash \lambda x : \forall \beta . \forall \alpha. \alpha \rightarrow \beta. (\Lambda \alpha. \Lambda \beta ((x\{\beta\})\{\alpha\})): (\forall \beta . \forall \alpha . \alpha \rightarrow \beta) \rightarrow (\forall \alpha. \forall \beta. \alpha \rightarrow \beta) } [t-abs]
\]

\newpage

\item

erase(f) \\
= erase($\lambda x : \forall \alpha . \forall \beta. \alpha \rightarrow \beta. (\Lambda \beta. \Lambda \alpha ((x\{\alpha\})\{\beta\}))$) \\
= $\lambda x$ . erase$(\Lambda \beta. \Lambda \alpha ((x\{\alpha\})\{\beta\})$) \\
= $\lambda x$ . erase$(\Lambda \alpha ((x\{\alpha\})\{\beta\})$) \\
= $\lambda x$ . erase$((x\{\alpha\})\{\beta\}$) \\
= $\lambda x$ . erase$(x\{\alpha\})$ \\
= $\lambda x$ . erase$(x)$ \\
= $\lambda x$ . x \\

erase(g) \\
= erase($\lambda x : \forall \beta. \forall \alpha. \alpha \rightarrow \beta. (\Lambda \alpha. \Lambda \beta ((x\{\beta\})\{\alpha\}))$) \\
= $\lambda x$ . erase$(\Lambda \alpha. \Lambda \beta ((x\{\beta\})\{\alpha\})$) \\
= $\lambda x$ . erase$(\Lambda \beta ((x\{\beta\})\{\alpha\})$) \\
= $\lambda x$ . erase$((x\{\beta\})\{\alpha\}$) \\
= $\lambda x$ . erase$(x\{\beta\})$ \\
= $\lambda x$ . erase$(x)$ \\
= $\lambda x$ . x \\

\item Two types f and g are equivalent if erase(f) $=_{\alpha}$ erase(g)

\item

\end{enumerate}

$a\left( \left( hmmm \right) \right)$
\end{document}
